README.md
@@ -1,2 +1,7 @@
 # formal_logic
-A formalization of formal logic in Lean
+
+A formalization of formal logic in Lean.
+
+This is built on top of the master branch of mathlib. 
+
+These theories are experimental and still under development.
